theories/typing/immovable.v
@@ -1,6 +1,6 @@
 From refinedc.typing Require Export type.
 From refinedc.typing Require Import programs.
-Set Default Proof Using "Type".
+From refinedc.typing Require Import type_options.
 
 Section immovable.
   Context `{!typeG Σ}.
